spinlock/SpinLockMainIAProof.v
@@ -34,7 +34,8 @@ Module SpinLockMainIA. Section SpinLockMainIA.
     init_simF u_a 0.
     (* process src precondition *)
     steps_l. iDestruct "ASM" as "[[-> [TID [%γ_l [#I F]]]] ->]". hss.
-    rename q2 into γ_v, q4 into ofs_v, q6 into blk_v, q8 into ofs_l, q10 into blk_l, q9 into tid.
+    destruct q4 as [blk_v ofs_v], q6 as [blk_l ofs_l]. 
+    rename q2 into γ_v, q5 into tid.
     (* main code *)
     steps_l. hss. steps_l. rewrite /SpinLockMainA.incr. steps_l.
     steps_r. hss. steps_r. rewrite /SpinLockMainI.incr. steps_r.
@@ -45,7 +46,7 @@ Module SpinLockMainIA. Section SpinLockMainIA.
     steps_r. sch_yield_r; iFrame.
     clear st_s st_t NODS NODD nths; iIntros (nths st_s st_t NODS NODD) "IST TID".
     (* tgt inline - lock acquire *)
-    inline_r. force_r (tid, γ_l, Vptr blk_l ofs_l, existT 0 (lock_P (blk_v, ofs_v) γ_v)).
+    inline_r. force_r (tid, γ_l, Vptr (blk_l, ofs_l), existT 0 (lock_P (blk_v, ofs_v) γ_v)).
     steps_r. forces_r. iFrame.
     iSplit; eauto. hss. steps_r.
     sch_yield_l. force_l false. steps_l.
@@ -85,7 +86,7 @@ Module SpinLockMainIA. Section SpinLockMainIA.
     iCombine "P F" as "C". iMod (own_update with "C") as "[F C]".
     { apply frac_auth_update, (Z_local_update _ _ (x + 1) 1); lia. }
     (* tgt inline - lock acquire - restore lock protected proposition *)
-    inline_r. force_r (tid, γ_l, Vptr blk_l ofs_l, existT 0 (lock_P (blk_v, ofs_v) γ_v)).
+    inline_r. force_r (tid, γ_l, Vptr (blk_l, ofs_l), existT 0 (lock_P (blk_v, ofs_v) γ_v)).
     forces_r.
     iSplitL "TID F PT TKN".
     { SL_red. rewrite /lock_P; ss. iSplit; iFrame; eauto. iSplit; eauto. iSplit.
@@ -138,8 +139,8 @@ Module SpinLockMainIA. Section SpinLockMainIA.
     sch_yield_r. iFrame; reintro nths. iIntros "IST".
     steps_r. iDestruct "GRT" as "[[TID [%val [%γ_l [-> #I]]]] %EQ]". hss. steps_r.
     sch_yield_r. iFrame; reintro nths. iIntros "IST TID".
-    iPoseProof "I" as "[%b_l [%o_l [-> _]]]".
-    sch_yield_l. steps_l. force_l (Vptr b_l o_l, Vptr blk 0). steps_l. sch_yield_l.
+    iPoseProof "I" as "[%bofs_l [-> _]]".
+    sch_yield_l. steps_l. force_l (Vptr bofs_l, Vptr (blk, 0%Z)). steps_l. sch_yield_l.
     (* create preconditions of incr *)
     iDestruct "W" as "[W1 W2]".
     (* spawn thread 1 - incr *)
@@ -181,7 +182,7 @@ Module SpinLockMainIA. Section SpinLockMainIA.
     iFrame; ss; clear nths st_s st_t NODS NODD; iIntros (nths st_s st_t NODS NODD) "IST TID".
     sch_yield_l. force_l false. steps_l.
     (* tgt inline - lock acquire *)
-    inline_r. force_r (0, γ_l, Vptr b_l o_l, existT 0 (lock_P (blk, 0%Z) γ)). forces_r. iFrame.
+    inline_r. force_r (0, γ_l, Vptr bofs_l, existT 0 (lock_P (blk, 0%Z) γ)). forces_r. iFrame.
     iSplit; eauto.
     steps_r. hss. steps_r.
     (* start coinduction for lock acquisition *)
@@ -199,8 +200,6 @@ Module SpinLockMainIA. Section SpinLockMainIA.
   iApply wsim_progress. iApply wsim_base_t.
   iSpecialize ("CIH" $! _).
   (hrepeat do 1 unshelve first[instantiate (1:= (_,_))|instantiate (1:= existT _ _)]); [..|s; grind; iIntrosFresh "I"; iApply "CIH"]; try eassumption.
-
-
       hss. iFrame. eauto.
     }
     (* success case *)
@@ -215,7 +214,7 @@ Module SpinLockMainIA. Section SpinLockMainIA.
     sch_yield_r. iFrame; reintro nths. iIntros "IST TID".
     sch_yield_r. iFrame; reintro nths. iIntros "IST TID".
     (* tgt inline - lock release *)
-    inline_r. force_r (0, γ_l, Vptr b_l o_l, existT 0 (lock_P (blk, 0%Z) γ)). forces_r.
+    inline_r. force_r (0, γ_l, Vptr bofs_l, existT 0 (lock_P (blk, 0%Z) γ)). forces_r.
     iSplitL "TKN TID B PT".
     { SL_red. iSplit; eauto. iFrame. iSplit; eauto. iSplit; eauto. iExists _; SL_red; iFrame. }
     steps_r. hss. steps_r.
